removing simp

theory/rBPFCommType.thy
@@ -4,6 +4,10 @@ imports
   "Word_Lib.Signed_Words"
 begin
 
+named_theorems bits_more_simp
+
+named_theorems list_more_simp
+
 type_synonym u4 = "4 word"
 type_synonym u8 = "8 word"
 type_synonym i8 = "8 sword"
@@ -76,8 +80,8 @@ definition arsh32 :: "i32 \<Rightarrow> nat \<Rightarrow> i32" where
 definition arsh64 :: "i64 \<Rightarrow> nat \<Rightarrow> i64" where
 "arsh64 x n = (if bit x 63 then or (drop_bit n x) (((2^n) -1) << 64-n) else drop_bit n x)"
 
-definition unsigned_bitfield_extract_u8 :: "nat \<Rightarrow> nat \<Rightarrow> u8 \<Rightarrow> u8" where
-"unsigned_bitfield_extract_u8 pos width n = and ((2 ^ width) - 1) (n >> pos)"
+definition bitfield_extract_u8 :: "nat \<Rightarrow> nat \<Rightarrow> u8 \<Rightarrow> u8" where
+"bitfield_extract_u8 pos width n = and ((2 ^ width) - 1) (n >> pos)"
 
 definition bitfield_insert_u8 :: "nat \<Rightarrow> nat \<Rightarrow> u8 \<Rightarrow> u8 \<Rightarrow> u8" where
 "bitfield_insert_u8 pos width n p = (
@@ -187,9 +191,9 @@ definition u16_of_u8_list :: "u8 list \<Rightarrow> u16 option" where
       )))
   )"
 
-lemma [simp]: "u8_of_bool False = 0" by (unfold u8_of_bool_def, simp)
+lemma u8_of_bool_false : "u8_of_bool False = 0" by (unfold u8_of_bool_def, simp)
 
-lemma [simp]: "u8_of_bool True = 1" by (unfold u8_of_bool_def, simp)
+lemma u8_of_bool_true : "u8_of_bool True = 1" by (unfold u8_of_bool_def, simp)
 
 
 lemma u8_ge_8_bit_false : "n \<ge> 8 \<Longrightarrow> \<not>bit (v::u8) n"
