theory/x86CommType.thy
@@ -71,8 +71,9 @@ definition construct_rex_to_u8 :: "bool\<Rightarrow> bool \<Rightarrow> bool \<R
 definition construct_modsib_to_u8 :: "u8 \<Rightarrow> u8 \<Rightarrow> u8 \<Rightarrow> u8" where
 "construct_modsib_to_u8 op1 op2 op3 =
   bitfield_insert_u8 6 2
-    (bitfield_insert_u8 3 3 (and 0b111 op3) (and 0b111 op2))
+    (bitfield_insert_u8 3 3
+      (bitfield_extract_u8 0 3 op3)
+      (bitfield_extract_u8 0 3 op2))
     op1"
-
 
 end
