theory/BitsLemma.thy
@@ -4,7 +4,9 @@ imports
   rBPFCommType
 begin
 
-lemma bits_zero_ext_u8 [simp]: " 0 \<le> i \<Longrightarrow>
+named_theorems bitfield_simps
+
+lemma bits_zero_ext_u8 [bitfield_simps]: " 0 \<le> i \<Longrightarrow>
   bit (and ((2 ^ n) - 1) (x::u8)) i = (if i < n then bit x i else False)"
   apply (induct_tac n, simp_all add: bit_simps)
   by (smt (verit) bit_1_0 bit_iff_odd bit_imp_le_length
@@ -12,11 +14,11 @@ lemma bits_zero_ext_u8 [simp]: " 0 \<le> i \<Longrightarrow>
       even_mult_exp_div_word_iff less_antisym mult.right_neutral
       not_less one_add_one power.simps(2) square_diff_one_factored)
 
-lemma bits_shl_u8 [simp]: "0 \<le> i \<Longrightarrow> i < 8 \<Longrightarrow>
+lemma bits_shl_u8 [bitfield_simps]: "0 \<le> i \<Longrightarrow> i < 8 \<Longrightarrow>
   bit ((x::u8) << y) i = (if i < y then False else bit x (i - y))"
   by (cases "i < y", simp_all add: bit_simps)
 
-lemma bits_mod_two_p_u8 [simp]: "0 \<le> n \<Longrightarrow> 0 \<le> i \<Longrightarrow>
+lemma bits_mod_two_p_u8 [bitfield_simps]: "0 \<le> n \<Longrightarrow> 0 \<le> i \<Longrightarrow>
   bit ((x::u8) mod (2 ^ n)) i = (if i < n then bit x i else False)"
   apply (induction n arbitrary: x i, simp_all add: bit_simps)
   subgoal for n x i
@@ -38,7 +40,11 @@ lemma mod_unique_u8: "\<And>(a::u8) b q r. r < b \<Longrightarrow>
     value "10 * (((10::u8) * 30 + 1) div 10)"
 *)
 
-lemma bits_two_p_m1_u8 [simp]: "n \<le> 8 \<Longrightarrow>
+lemma bit_2_power_n_ge_False [bitfield_simps]: " i \<ge> n \<Longrightarrow> bit ((2 ^ n - 1)::u8) i = False"
+  by (simp add: bit_iff_odd even_mask_div_iff)
+
+
+lemma bits_two_p_m1_u8 [bitfield_simps]: "n \<le> 8 \<Longrightarrow>
   bit ((2 ^ n - 1)::u8) i = (if i < n then True else False)"
   apply (cases n, simp_all add: bit_simps)
   subgoal for n1 apply (cases n1, simp_all add: bit_simps)
@@ -112,21 +118,21 @@ lemma bits_two_p_m1_u8 [simp]: "n \<le> 8 \<Longrightarrow>
     done
   done
 
-lemma bits_unsigned_bitfield_extract_u8: "
+lemma bis_bitfield_extract_u8 [bitfield_simps]: "
   0 \<le> pos \<Longrightarrow> 0 < width \<Longrightarrow> pos + width \<le> 8 \<Longrightarrow>
   0 \<le> i \<Longrightarrow> i < 8 \<Longrightarrow> \<comment> \<open> TODO: i \<le> 8 is also OK !!  \<close>
-  bit (unsigned_bitfield_extract_u8 pos width n) i =
+  bit (bitfield_extract_u8 pos width n) i =
   (if i < width then bit n (i + pos) else False)"
-  apply (unfold unsigned_bitfield_extract_u8_def)
+  apply (unfold bitfield_extract_u8_def)
   apply (simp only: bits_zero_ext_u8)
   apply (cases "i < width", simp_all add: bit_simps)
   apply (simp add: add.commute)
   done
 
-lemma [simp]: "\<not> (i::nat) < pos \<Longrightarrow> (i - pos < width) = (i < pos + width)"
+lemma nat_ge_minus_eq : "\<not> (i::nat) < pos \<Longrightarrow> (i - pos < width) = (i < pos + width)"
   by (simp add: add.commute less_diff_conv2)
 
-lemma bits_bitfield_insert_u8: "
+lemma bits_bitfield_insert_u8 [bitfield_simps]: "
   0 \<le> pos \<Longrightarrow> 0 < width \<Longrightarrow> pos + width \<le> 8 \<Longrightarrow>
   0 \<le> i \<Longrightarrow> i < 8 \<Longrightarrow>
   bit (bitfield_insert_u8 pos width n p) i =
@@ -137,12 +143,66 @@ lemma bits_bitfield_insert_u8: "
   apply (simp only: bit_not_iff)
   apply (simp only: bits_shl_u8)
   apply (simp only: bits_zero_ext_u8)
-  apply (cases "i < pos", simp_all)
+  apply (cases "i < pos"; simp add: bits_two_p_m1_u8 nat_ge_minus_eq)
   done
 
 subsection \<open> So we may be use
 - `bits_unsigned_bitfield_extract_u8` and 
 - `bits_bitfield_insert_u8`
  to implement ops for u16/u32/u64 \<close>
+
+lemma bitfield_extract_insert_same0 [bitfield_simps]:
+  "0 < w0 \<Longrightarrow> p0 + w0 \<le> 8 \<Longrightarrow>
+  bitfield_extract_u8 p0 w0 (bitfield_insert_u8 p0 w0 n v) =
+  bitfield_extract_u8 0 w0 v"
+  apply (simp add: bit_eq_iff)
+  apply (rule allI)
+  subgoal by (simp add: bitfield_simps)
+  done
+
+lemma bitfield_extract_insert_same1 [bitfield_simps]:
+  "0 < w0 \<Longrightarrow> 0 < w1 \<Longrightarrow> p0 + w0 \<le> p1 \<Longrightarrow> p1 + w1 \<le> 8 \<Longrightarrow>
+  bitfield_extract_u8 p0 w0 (bitfield_insert_u8 p1 w1 n v) =
+  bitfield_extract_u8 p0 w0 n"
+  apply (simp add: bit_eq_iff)
+  apply (rule allI)
+  subgoal by (simp add: bitfield_simps)
+  done
+
+lemma bitfield_extract_same_0 [bitfield_simps]:
+  "0 < w0 \<Longrightarrow> p0 + w0 < 8 \<Longrightarrow>
+    bitfield_extract_u8 0 w0 (bitfield_extract_u8 p0 w0 v) =
+    bitfield_extract_u8 p0 w0 v"
+  apply (simp add: bit_eq_iff)
+  apply (rule allI)
+  subgoal by (simp add: bitfield_simps)
+  done
+
+lemma bitfield_extract_u8_width_1 [bitfield_simps]:
+  " bitfield_extract_u8 p0 1 v = 0 \<or>
+    bitfield_extract_u8 p0 1 v = 1"
+  apply (simp add: bitfield_extract_u8_def)
+  by (metis not_mod_2_eq_0_eq_1 one_and_eq)
+
+lemma bitfield_extract_u8_of_bool_same [bitfield_simps]:
+  "p0 < 7 \<Longrightarrow>
+    u8_of_bool (bitfield_extract_u8 p0 (Suc 0) v \<noteq> 0) =
+    bitfield_extract_u8 p0 1 v"
+  apply (unfold u8_of_bool_def)
+  apply (cases "bitfield_extract_u8 p0 1 v \<noteq> 0"; simp)
+  using bitfield_extract_u8_width_1 by fastforce
+
+lemma bitfield_insert_extract_same0 [bitfield_simps]:
+  " 0 < w0 \<Longrightarrow> 0 < w1 \<Longrightarrow> w0 + w1 < 8 \<Longrightarrow>
+    bitfield_insert_u8 w0 w1
+     (bitfield_extract_u8 0 w0 v)
+     (bitfield_extract_u8 w0 w1 v) =
+    bitfield_extract_u8 0 (w0+w1) v"
+  apply (simp add: bit_eq_iff)
+  apply (rule allI)
+  subgoal for n
+    apply (simp add: bitfield_simps)
+    by linarith
+  done
 
 end
