theory/BitsOpMore.thy
@@ -5,12 +5,12 @@ imports
   x64Syntax
 begin
 
-lemma [simp]: "and (and (and 7 (v::u8)) (- 9)) 8 = 0"
+lemma and_3_7_8 [bits_more_simp]: "and (and (and 7 (v::u8)) (- 9)) 8 = 0"
   apply (simp add: bit_eq_iff)
   apply (auto simp add: bit_simps)
   done
 
-lemma [simp]: "(and (and 7 (k::u8)) (- 9)) = and 7 k"
+lemma and_2_7_minus_9 [bits_more_simp]: "(and (and 7 (k::u8)) (- 9)) = and 7 k"
   apply (simp add: bit_eq_iff)
   apply (auto simp add: bit_simps)
   subgoal for n apply (cases n, simp_all)
@@ -24,7 +24,7 @@ lemma [simp]: "(and (and 7 (k::u8)) (- 9)) = and 7 k"
 lemma and_1_eq_1: "\<And> v. (and 1 v \<noteq> 0) = (and 1 v = 1)"
   by (simp add: one_and_eq)
 
-lemma [simp]: "and 1 ((v::u8) >> 2) = 1 \<Longrightarrow> (and 8 ((v >> 2) << 3) = 8)"
+lemma and_1_shr_2_1 [bits_more_simp]: "and 1 ((v::u8) >> 2) = 1 \<Longrightarrow> (and 8 ((v >> 2) << 3) = 8)"
   apply (simp add: bit_eq_iff)
   apply (auto simp add: bit_simps)
   subgoal for k
@@ -41,7 +41,7 @@ lemma [simp]: "and 1 ((v::u8) >> 2) = 1 \<Longrightarrow> (and 8 ((v >> 2) << 3)
     done
   done
 
-lemma [simp]: "and 1 (v >> 2) = 1 \<Longrightarrow> and (or (and 8 (((v::u8) >> 2) << 3)) (and (and 7 (k >> 3)) (- 9))) 8 \<noteq> 0"
+lemma and_1_shr_2_1_neq_0 [bits_more_simp]: "and 1 (v >> 2) = 1 \<Longrightarrow> and (or (and 8 (((v::u8) >> 2) << 3)) (and (and 7 (k >> 3)) (- 9))) 8 \<noteq> 0"
   apply (simp add: bit_eq_iff)
   apply (auto simp add: bit_simps)
   apply (rule_tac x="3" in exI)
@@ -49,7 +49,7 @@ lemma [simp]: "and 1 (v >> 2) = 1 \<Longrightarrow> and (or (and 8 (((v::u8) >> 
   apply simp
   done
 
-lemma [simp]: "and (and 7 (v::u8)) 8 = 0"
+lemma and_2_7_8_0 [bits_more_simp]: "and (and 7 (v::u8)) 8 = 0"
   apply (simp add: bit_eq_iff)
   apply (auto simp add: bit_simps)
   subgoal for n apply (cases n, simp_all)
@@ -60,7 +60,7 @@ lemma [simp]: "and (and 7 (v::u8)) 8 = 0"
     done
   done
 
-lemma [simp]: "and (or (and 8 (v::u8)) (and 7 k)) 8 = and 8 v"
+lemma and_or_and_8_7_8 [bits_more_simp]: "and (or (and 8 (v::u8)) (and 7 k)) 8 = and 8 v"
   apply (simp add: bit_eq_iff)
   apply (auto simp add: bit_simps)
   subgoal for n apply (cases n, simp_all)
@@ -71,43 +71,43 @@ lemma [simp]: "and (or (and 8 (v::u8)) (and 7 k)) 8 = and 8 v"
     done
   done
 
-lemma [simp]: "and 15 ((v::u8) >> 4) = 4 \<Longrightarrow> bit v (Suc (Suc (Suc (Suc (Suc 0))))) = False"
+lemma and_15_shr_4_4_false0 [bits_more_simp]: "and 15 ((v::u8) >> 4) = 4 \<Longrightarrow> bit v (Suc (Suc (Suc (Suc (Suc 0))))) = False"
   apply (simp add: bit_eq_iff)
   apply (auto simp add: bit_simps)
   apply (drule_tac x="1" in spec)
   apply simp
   by (simp add: numeral_eq_Suc)
 
-lemma [simp]: "and 15 ((v::u8) >> 4) = 4 \<Longrightarrow> bit v (Suc (Suc (Suc (Suc (Suc (Suc 0)))))) = True"
+lemma and_15_shr_4_4_true [bits_more_simp]: "and 15 ((v::u8) >> 4) = 4 \<Longrightarrow> bit v (Suc (Suc (Suc (Suc (Suc (Suc 0)))))) = True"
   apply (simp add: bit_eq_iff)
   apply (auto simp add: bit_simps)
   apply (drule_tac x="2" in spec)
   apply simp
   by (simp add: numeral_eq_Suc)
 
-lemma [simp]: "and 15 ((v::u8) >> 4) = 4 \<Longrightarrow> bit v (Suc (Suc (Suc (Suc (Suc (Suc (Suc 0))))))) = False"
+lemma and_15_shr_4_4_false1 [bits_more_simp]: "and 15 ((v::u8) >> 4) = 4 \<Longrightarrow> bit v (Suc (Suc (Suc (Suc (Suc (Suc (Suc 0))))))) = False"
   apply (simp add: bit_eq_iff)
   apply (auto simp add: bit_simps)
   apply (drule_tac x="3" in spec)
   apply simp
   by (simp add: numeral_eq_Suc)
 
-lemma [simp]: "(and 1 ((v::u8) >> n) = 1) = (bit v n = True)"
+lemma and_1_shr_n_1 [bits_more_simp]: "(and 1 ((v::u8) >> n) = 1) = (bit v n = True)"
   apply (simp add: bit_eq_iff)
   apply (auto simp add: bit_simps)
   apply (drule_tac x="0" in spec)
     by (simp add: numeral_2_eq_2)
 
-lemma [simp]: "(and 1 ((v::u8) >> n) = 0) = (bit v n = False)"
+lemma and_1_shr_n_0 [bits_more_simp]: "(and 1 ((v::u8) >> n) = 0) = (bit v n = False)"
   apply (simp add: bit_eq_iff)
   apply (auto simp add: bit_simps)
   apply (drule_tac x="0" in spec)
     by (simp add: numeral_2_eq_2)
 
-lemma [simp]: "bit v 2 \<Longrightarrow> bit v (Suc (Suc 0))"
+lemma bit_v_2 [bits_more_simp]: "bit v 2 \<Longrightarrow> bit v (Suc (Suc 0))"
  using numeral_2_eq_2 by argo
 
-lemma [simp]: "\<not> bit (7::int) n \<Longrightarrow> 3 \<le> n"
+lemma bit_7_3_lt [bits_more_simp]: "\<not> bit (7::int) n \<Longrightarrow> 3 \<le> n"
   apply (cases n, simp_all)
   subgoal for n1 apply (cases n1, simp_all)
     subgoal for n2 apply (cases n2, simp_all)
@@ -115,7 +115,7 @@ lemma [simp]: "\<not> bit (7::int) n \<Longrightarrow> 3 \<le> n"
     done
   done
 
-lemma [simp]: "bit (56::int) n \<Longrightarrow> 3 \<le> n"
+lemma bit_56_3_le [bits_more_simp]: "bit (56::int) n \<Longrightarrow> 3 \<le> n"
   apply (cases n, simp_all)
   subgoal for n1 apply (cases n1, simp_all)
     subgoal for n2 apply (cases n2, simp_all)
@@ -123,7 +123,7 @@ lemma [simp]: "bit (56::int) n \<Longrightarrow> 3 \<le> n"
     done
   done
 
-lemma and_3_shr_6_1_False [simp]: "and 3 ((v::u8) >> 6) = 1 \<Longrightarrow>
+lemma and_3_shr_6_1_False [bits_more_simp]: "and 3 ((v::u8) >> 6) = 1 \<Longrightarrow>
     bit v (Suc (Suc (Suc (Suc (Suc (Suc (Suc 0))))))) \<Longrightarrow> False"
   apply (simp only: bit_eq_iff)
   apply (auto simp add: bit_simps)
@@ -141,7 +141,7 @@ lemma not_7_lt_3 [simp]: "\<not> bit (7::int) n \<Longrightarrow> \<not> 3 \<le>
     done
   done *)
 
-lemma and_8_shl_3_neq_0 [simp]: "(and 8 ((v::u8) << 3) \<noteq> 0) = (bit v 0 = True)"
+lemma and_8_shl_3_neq_0 [bits_more_simp]: "(and 8 ((v::u8) << 3) \<noteq> 0) = (bit v 0 = True)"
   apply (simp add: bit_eq_iff)
   apply (auto simp add: bit_simps)
   subgoal for n apply (cases n, simp_all)
@@ -159,7 +159,7 @@ lemma and_8_shl_3_neq_0 [simp]: "(and 8 ((v::u8) << 3) \<noteq> 0) = (bit v 0 = 
     done
   done
 
-lemma encode_movl_rr_1_subgoal_1 [simp]: "n < 8 \<Longrightarrow> 
+lemma encode_movl_rr_1_subgoal_1 [bits_more_simp]: "n < 8 \<Longrightarrow> 
   \<not> bit (192::int) n \<Longrightarrow> \<not> bit (7::int) n \<Longrightarrow> bit (56::int) n"
   apply (cases n, simp_all)
   subgoal for n1 apply (cases n1, simp_all)
@@ -176,7 +176,7 @@ lemma encode_movl_rr_1_subgoal_1 [simp]: "n < 8 \<Longrightarrow>
     done
   done
 
-lemma encode_movl_rr_1_subgoal_2 [simp]: "n < 8 \<Longrightarrow> 
+lemma encode_movl_rr_1_subgoal_2 [bits_more_simp]: "n < 8 \<Longrightarrow> 
   \<not> bit (192::int) n \<Longrightarrow> \<not> bit (7::int) n \<Longrightarrow> 3 \<le> n"
   apply (cases n, simp_all)
   subgoal for n1 apply (cases n1, simp_all)
@@ -186,7 +186,7 @@ lemma encode_movl_rr_1_subgoal_2 [simp]: "n < 8 \<Longrightarrow>
   done
 
 
-lemma encode_movl_rr_1_subgoal_3 [simp]: "n < 8 \<Longrightarrow> 
+lemma encode_movl_rr_1_subgoal_3 [bits_more_simp]: "n < 8 \<Longrightarrow> 
   \<not> bit (192::int) n \<Longrightarrow> \<not> bit (7::int) n \<Longrightarrow> bit (71::int) n \<Longrightarrow> False"
   apply (cases n, simp_all)
   subgoal for n1 apply (cases n1, simp_all)
@@ -203,7 +203,7 @@ lemma encode_movl_rr_1_subgoal_3 [simp]: "n < 8 \<Longrightarrow>
     done
   done
 
-lemma encode_movl_rr_1_subgoal_4 [simp]: "n < 8 \<Longrightarrow>
+lemma encode_movl_rr_1_subgoal_4 [bits_more_simp]: "n < 8 \<Longrightarrow>
   \<not> bit (192::int) n \<Longrightarrow> \<not> bit (56::int) n \<Longrightarrow> bit (8::int) n \<Longrightarrow> False"
   apply (cases n, simp_all)
   subgoal for n1 apply (cases n1, simp_all)
@@ -214,7 +214,7 @@ lemma encode_movl_rr_1_subgoal_4 [simp]: "n < 8 \<Longrightarrow>
     done
   done
 
-lemma encode_movl_rr_1_subgoal_5 [simp]:
+lemma encode_movl_rr_1_subgoal_5 [bits_more_simp]:
   "\<not> bit (192::int) n \<Longrightarrow> \<not> 3 \<le> n \<Longrightarrow> bit (8::int) n \<Longrightarrow> False"
   apply (cases n, simp_all)
   subgoal for n1 apply (cases n1, simp_all)
@@ -223,7 +223,7 @@ lemma encode_movl_rr_1_subgoal_5 [simp]:
     done
   done
 
-lemma encode_movl_rr_1_subgoal_6 [simp]:
+lemma encode_movl_rr_1_subgoal_6 [bits_more_simp]:
   "\<not> bit (192::int) n \<Longrightarrow> \<not> 3 \<le> n \<Longrightarrow> bit (56::int) n \<Longrightarrow> False"
   apply (cases n, simp_all)
   subgoal for n1 apply (cases n1, simp_all)
@@ -232,7 +232,7 @@ lemma encode_movl_rr_1_subgoal_6 [simp]:
     done
   done
 
-lemma encode_movl_rr_1_subgoal_7 [simp]: "n < 8 \<Longrightarrow> bit (v::u8) n \<Longrightarrow>
+lemma encode_movl_rr_1_subgoal_7 [bits_more_simp]: "n < 8 \<Longrightarrow> bit (v::u8) n \<Longrightarrow>
   \<not> bit (192::int) n \<Longrightarrow> bit (8::int) n \<Longrightarrow> bit v (3 + (n - 3))"
   apply (cases n, simp_all)
   subgoal for n1 apply (cases n1, simp_all)
@@ -243,7 +243,7 @@ lemma encode_movl_rr_1_subgoal_7 [simp]: "n < 8 \<Longrightarrow> bit (v::u8) n 
     done
   done
 
-lemma encode_movl_rr_1_subgoal_8[simp]: "n < 8 \<Longrightarrow>
+lemma encode_movl_rr_1_subgoal_8[bits_more_simp]: "n < 8 \<Longrightarrow>
   \<not> bit (192::int) n \<Longrightarrow> bit (8::int) n \<Longrightarrow> bit (71::int) n \<Longrightarrow> False"
   apply (cases n, simp_all)
   subgoal for n1 apply (cases n1, simp_all)
@@ -254,7 +254,7 @@ lemma encode_movl_rr_1_subgoal_8[simp]: "n < 8 \<Longrightarrow>
     done
   done
 
-lemma encode_movl_rr_1_subgoal_9 [simp]: "n < 8 \<Longrightarrow> bit (v::u8) n \<Longrightarrow>
+lemma encode_movl_rr_1_subgoal_9 [bits_more_simp]: "n < 8 \<Longrightarrow> bit (v::u8) n \<Longrightarrow>
   \<not> bit (192::int) n \<Longrightarrow> bit (56::int) n \<Longrightarrow> bit v (3 + (n - 3))"
   apply (cases n, simp_all)
   subgoal for n1 apply (cases n1, simp_all)
@@ -272,7 +272,7 @@ lemma encode_movl_rr_1_subgoal_9 [simp]: "n < 8 \<Longrightarrow> bit (v::u8) n 
     done
   done
 
-lemma encode_movl_rr_1_subgoal_10 [simp]: "n < 8 \<Longrightarrow>
+lemma encode_movl_rr_1_subgoal_10 [bits_more_simp]: "n < 8 \<Longrightarrow>
   \<not> bit (192::int) n \<Longrightarrow> bit (56::int) n \<Longrightarrow> bit (71::int) n \<Longrightarrow> False"
   apply (cases n, simp_all)
   subgoal for n1 apply (cases n1, simp_all)
@@ -287,10 +287,10 @@ lemma encode_movl_rr_1_subgoal_10 [simp]: "n < 8 \<Longrightarrow>
     done
   done
 
-lemma and_3_shr_6_3_6 [simp]: "and 3 (v >> 6) = 3 \<Longrightarrow> bit v (Suc (Suc (Suc (Suc (Suc (Suc 0))))))"
+lemma and_3_shr_6_3_6 [bits_more_simp]: "and 3 (v >> 6) = 3 \<Longrightarrow> bit v (Suc (Suc (Suc (Suc (Suc (Suc 0))))))"
   by (metis Suc3_eq_add_3 bit_0 bit_and_iff bit_iff_odd_drop_bit bit_numeral_Bit1_0 numeral_3_eq_3 numeral_Bit0)
 
-lemma and_3_shr_6_3_7 [simp]: "and 3 ((v::u8) >> 6) = 3 \<Longrightarrow> bit v (Suc (Suc (Suc (Suc (Suc (Suc (Suc 0)))))))"
+lemma and_3_shr_6_3_7 [bits_more_simp]: "and 3 ((v::u8) >> 6) = 3 \<Longrightarrow> bit v (Suc (Suc (Suc (Suc (Suc (Suc (Suc 0)))))))"
   apply (simp add: bit_eq_iff)
   apply (auto simp add: bit_simps)
   apply (drule_tac x="1" in spec)
@@ -298,7 +298,7 @@ lemma and_3_shr_6_3_7 [simp]: "and 3 ((v::u8) >> 6) = 3 \<Longrightarrow> bit v 
   done
 
 
-lemma encode_movl_rr_1_subgoal_11 [simp]: "and 3 (v >> 6) = 3 \<Longrightarrow>
+lemma encode_movl_rr_1_subgoal_11 [bits_more_simp]: "and 3 (v >> 6) = 3 \<Longrightarrow>
   u8_of_ireg src = and (and 7 (v >> 3)) (- 9) \<Longrightarrow> u8_of_ireg dst = and (and 7 v) (- 9) \<Longrightarrow>
   n < 8 \<Longrightarrow> bit (192::int) n \<Longrightarrow> bit v n"
   apply (cases n, simp_all)
@@ -307,7 +307,7 @@ lemma encode_movl_rr_1_subgoal_11 [simp]: "and 3 (v >> 6) = 3 \<Longrightarrow>
       subgoal for n3 apply (cases n3, simp_all)
         subgoal for n4 apply (cases n4, simp_all)
           subgoal for n5 apply (cases n5, simp_all)
-            subgoal for n6 apply (cases n6, simp_all)
+            subgoal for n6 apply (cases n6, simp_all add: bits_more_simp)
               done
             done
           done
@@ -316,14 +316,14 @@ lemma encode_movl_rr_1_subgoal_11 [simp]: "and 3 (v >> 6) = 3 \<Longrightarrow>
     done
   done
 
-lemma encode_movl_rr_1_subgoal_12 [simp]: "and 3 ((k::u8) >> 6) = 3 \<Longrightarrow> n < 8 \<Longrightarrow> bit 192 n \<Longrightarrow> bit k n"
+lemma encode_movl_rr_1_subgoal_12 [bits_more_simp]: "and 3 ((k::u8) >> 6) = 3 \<Longrightarrow> n < 8 \<Longrightarrow> bit 192 n \<Longrightarrow> bit k n"
   apply (cases n, simp_all)
   subgoal for n1 apply (cases n1, simp_all add: bit_numeral_Bit0_iff) 
     subgoal for n2 apply (cases n2, simp_all)
       subgoal for n3 apply (cases n3, simp_all)
         subgoal for n4 apply (cases n4, simp_all)
           subgoal for n5 apply (cases n5, simp_all)
-            subgoal for n6 apply (cases n6, simp_all)
+            subgoal for n6 apply (cases n6, simp_all add: bits_more_simp)
               done
             done
           done
@@ -332,7 +332,7 @@ lemma encode_movl_rr_1_subgoal_12 [simp]: "and 3 ((k::u8) >> 6) = 3 \<Longrighta
     done
   done
 
-lemma encode_movl_rr_1_subgoal_13 [simp]: "and 3 ((k::u8) >> 6) = 3 \<Longrightarrow> n < 8 \<Longrightarrow>
+lemma encode_movl_rr_1_subgoal_13 [bits_more_simp]: "and 3 ((k::u8) >> 6) = 3 \<Longrightarrow> n < 8 \<Longrightarrow>
   \<not> bit 192 n \<Longrightarrow> bit 56 n \<Longrightarrow> bit 64 n \<Longrightarrow> bit k n"
   apply (cases n, simp_all)
   subgoal for n1 apply (cases n1, simp_all add: bit_numeral_Bit0_iff) 
@@ -340,7 +340,7 @@ lemma encode_movl_rr_1_subgoal_13 [simp]: "and 3 ((k::u8) >> 6) = 3 \<Longrighta
       subgoal for n3 apply (cases n3, simp_all)
         subgoal for n4 apply (cases n4, simp_all)
           subgoal for n5 apply (cases n5, simp_all)
-            subgoal for n6 apply (cases n6, simp_all)
+            subgoal for n6 apply (cases n6, simp_all add: bits_more_simp)
               done
             done
           done
