theory/BitsOpMore2.thy
@@ -4,22 +4,11 @@ imports
   rBPFCommType 
 begin
 
-lemma ucast64_ucast8_and_255_eq [simp]: "ucast (((ucast (and v 255))::u8)) = and (v:: u64) 255"
-  apply (simp only: ucast_eq)
-(**r 
-word_of_int (uint (word_of_int (uint (and v 255)))) is
-
-(word_of_int (uint (and v 255)))::u8
-
-word_of_int (uint v_u8)  :: u64
-
-*)
-  apply (simp only: uint_word_of_int_eq word_and_def word_of_int_eq_iff)
-  apply (simp)
-  apply (simp add: bit_eq_iff)
-  apply (auto simp add: bit_simps)
-  subgoal for n
-    apply (cases n, simp_all)
+lemma ucast64_ucast8_and_255_eq [bits_more_simp]:
+"ucast (((ucast (and v 255))::u8)) = and (v:: u64) 255"
+  apply (simp only: ucast_eq uint_word_of_int_eq word_and_def word_of_int_eq_iff)
+  apply (auto simp add: bit_simps bit_eq_iff)
+  subgoal for n apply (cases n, simp_all)
     subgoal for n1 apply (cases n1, simp_all)
       subgoal for n2 apply (cases n2, simp_all)
         subgoal for n3 apply (cases n3, simp_all)
@@ -37,11 +26,9 @@ word_of_int (uint v_u8)  :: u64
     done
   done
 
-lemma u64_shl_shr_same : "n \<le> 56 \<Longrightarrow> ((ucast (v::u8) ::u64) << n) >> n = (ucast (v::u8) ::u64)"
-  apply (simp add: bit_eq_iff)
-  apply (auto simp add: bit_simps)
-  subgoal for k
-    apply (cases k, simp_all)
+lemma u64_shl_shr_same [bits_more_simp]: "n \<le> 56 \<Longrightarrow> ((ucast (v::u8) ::u64) << n) >> n = (ucast (v::u8) ::u64)"
+  apply (auto simp add: bit_simps bit_eq_iff)
+  subgoal for k apply (cases k, simp_all)
     subgoal for n1 apply (cases n1, simp_all)
       subgoal for n2 apply (cases n2, simp_all)
         subgoal for n3 apply (cases n3, simp_all)
@@ -59,32 +46,27 @@ lemma u64_shl_shr_same : "n \<le> 56 \<Longrightarrow> ((ucast (v::u8) ::u64) <<
     done
   done
 
-lemma u64_shl_shr_outside: "n+8 \<le> m \<Longrightarrow> ((ucast (v::u8) ::u64) << n) >> m = (0 ::u64)"
-  apply (simp add: bit_eq_iff)
-  apply (auto simp add: bit_simps u8_ge_8_bit_false)
-  done
+lemma u64_shl_shr_outside [bits_more_simp]: "n+8 \<le> m \<Longrightarrow> ((ucast (v::u8) ::u64) << n) >> m = (0 ::u64)"
+  by (auto simp add: bit_simps u8_ge_8_bit_false bit_eq_iff)
 
-lemma [simp]: "(n::nat) \<le> 56 \<Longrightarrow> m \<le> n \<Longrightarrow> k < 64 \<Longrightarrow> n - m \<le> k \<Longrightarrow> k + m - n < 8 \<Longrightarrow> m + k < 64"
+lemma nat_le_56 : "(n::nat) \<le> 56 \<Longrightarrow> m \<le> n \<Longrightarrow> k < 64 \<Longrightarrow> n - m \<le> k \<Longrightarrow> k + m - n < 8 \<Longrightarrow> m + k < 64"
   by simp
 
-lemma u64_shl_shr_same_minus: "n \<le> 56 \<Longrightarrow> m \<le> n \<Longrightarrow> ((ucast (v::u8) ::u64) << n) >> m =
+lemma u64_shl_shr_same_minus [bits_more_simp]: "n \<le> 56 \<Longrightarrow> m \<le> n \<Longrightarrow> ((ucast (v::u8) ::u64) << n) >> m =
   ((ucast (v::u8) ::u64) << (n-m))"
-  apply (simp add: bit_eq_iff)
-  apply (auto simp add: bit_simps u8_bit_true_ge_8)
+  apply (auto simp add: bit_simps u8_bit_true_ge_8 nat_le_56 bit_eq_iff)
   subgoal for k
     by (simp add: add.commute)
   subgoal for k
     by (metis add.commute)
   done
 
-lemma [simp]: "8 \<le> m \<Longrightarrow> (ucast (v::u8) ::u64) >> m = (0 ::u64)"
-  apply (simp add: bit_eq_iff)
-  apply (auto simp add: bit_simps u8_ge_8_bit_false)
+lemma u8_ge_8_ucast_0 [bits_more_simp]: "8 \<le> m \<Longrightarrow> (ucast (v::u8) ::u64) >> m = (0 ::u64)"
+  apply (auto simp add: bit_simps u8_ge_8_bit_false bit_eq_iff)
   done
 
-lemma u64_and_or_255_same: "8 \<le> n \<Longrightarrow> (and (or ((v::u64) << n) k) 255) = and k 255"
-  apply (simp add: bit_eq_iff)
-  apply (auto simp add: bit_simps)
+lemma u64_and_or_255_same [bits_more_simp]: "8 \<le> n \<Longrightarrow> (and (or ((v::u64) << n) k) 255) = and k 255"
+  apply (auto simp add: bit_simps bit_eq_iff)
   subgoal for t apply (cases t, simp_all)
     subgoal for n1 apply (cases n1, simp_all)
       subgoal for n2 apply (cases n2, simp_all)
@@ -103,12 +85,9 @@ lemma u64_and_or_255_same: "8 \<le> n \<Longrightarrow> (and (or ((v::u64) << n)
     done
   done
 
-lemma u64_ucast_and_ucast_255_same: "(ucast (and (ucast (v::u8)) (255::u64)) ::u8) = v"
-  apply (simp only: ucast_eq)
-  apply (simp only: uint_word_of_int_eq word_and_def word_of_int_eq_iff)
-  apply simp
-  apply (simp add: bit_eq_iff)
-  apply (auto simp add: bit_simps)
+lemma u64_ucast_and_ucast_255_same [bits_more_simp]: "(ucast (and (ucast (v::u8)) (255::u64)) ::u8) = v"
+  apply (simp only: ucast_eq uint_word_of_int_eq word_and_def word_of_int_eq_iff)
+  apply (auto simp add: bit_simps bit_eq_iff)
   subgoal for n apply (cases n, simp_all)
     subgoal for n1 apply (cases n1, simp_all)
       subgoal for n2 apply (cases n2, simp_all)
@@ -132,68 +111,58 @@ lemma list_consists_8 : "length l = 8 \<Longrightarrow>
       less_Suc_eq list.sel(3) nat_1_add_1
       semiring_norm(26) semiring_norm(27) semiring_norm(28) take0)
 
-lemma u64_ucast_ucast_and_shr_255_shl_same: "n \<le> 56 \<Longrightarrow>
+lemma u64_ucast_ucast_and_shr_255_shl_same [bits_more_simp]: "n \<le> 56 \<Longrightarrow>
   ((ucast ((ucast (and ((v::u64) >> n) 255)) ::u8) ::u64) << n) =
   ((and ((v::u64) >> n) 255) << n)"
-  apply (simp only: ucast_eq)
-  apply (simp only: uint_word_of_int_eq word_and_def word_of_int_eq_iff)
-  apply simp
-  apply (simp add: bit_eq_iff)
-  apply (auto simp add: bit_simps)
+  apply (simp only: ucast_eq uint_word_of_int_eq word_and_def word_of_int_eq_iff)
+  apply (auto simp add: bit_simps bit_eq_iff)
   subgoal for n1
   using bit_power_k_minus_1_le [of 8 "n1-n"] by simp
   done
 
-lemma [simp]: "and (((v::u64) >> 56) << 56) 18374686479671623680 = and v 18374686479671623680"
-  apply (simp add: bit_eq_iff)
-  apply (auto simp add: bit_simps)
+lemma u8_and_2_power_56_eq [bits_more_simp]: "and (((v::u64) >> 56) << 56) 18374686479671623680 = and v 18374686479671623680"
+  apply (auto simp add: bit_simps bit_eq_iff)
   subgoal for n using bit_power_k_add_m_ge [of 56 8 n] by simp
   subgoal for n using bit_power_k_add_m_ge [of 56 8 n] by simp
   done
 
-lemma [simp]: "and (((v::u64) >> 48) << 48) 71776119061217280 = and v 71776119061217280"
-  apply (simp add: bit_eq_iff)
-  apply (auto simp add: bit_simps)
+lemma u8_and_2_power_48_eq [bits_more_simp]: "and (((v::u64) >> 48) << 48) 71776119061217280 = and v 71776119061217280"
+  apply (auto simp add: bit_simps bit_eq_iff)
   subgoal for n using bit_power_k_add_m_ge [of 48 8 n] by simp
   subgoal for n using bit_power_k_add_m_ge [of 48 8 n] by simp
   done
 
-lemma [simp]: "and (((v::u64) >> 40) << 40) 280375465082880 = and v 280375465082880"
-  apply (simp add: bit_eq_iff)
-  apply (auto simp add: bit_simps)
+lemma u8_and_2_power_40_eq [bits_more_simp]: "and (((v::u64) >> 40) << 40) 280375465082880 = and v 280375465082880"
+  apply (auto simp add: bit_simps bit_eq_iff)
   subgoal for n using bit_power_k_add_m_ge [of 40 8 n] by simp
   subgoal for n using bit_power_k_add_m_ge [of 40 8 n] by simp
   done
 
-lemma [simp]: "and (((v::u64) >> 32) << 32) 1095216660480 = and v 1095216660480"
-  apply (simp add: bit_eq_iff)
-  apply (auto simp add: bit_simps)
+lemma u8_and_2_power_32_eq [bits_more_simp]: "and (((v::u64) >> 32) << 32) 1095216660480 = and v 1095216660480"
+  apply (auto simp add: bit_simps bit_eq_iff)
   subgoal for n using bit_power_k_add_m_ge [of 32 8 n] by simp
   subgoal for n using bit_power_k_add_m_ge [of 32 8 n] by simp
   done
 
-lemma [simp]: "and (((v::u64) >> 24) << 24) 4278190080 = and v 4278190080"
-  apply (simp add: bit_eq_iff)
-  apply (auto simp add: bit_simps)
+lemma u8_and_2_power_24_eq [bits_more_simp]: "and (((v::u64) >> 24) << 24) 4278190080 = and v 4278190080"
+  apply (auto simp add: bit_simps bit_eq_iff)
   subgoal for n using bit_power_k_add_m_ge [of 24 8 n] by simp
   subgoal for n using bit_power_k_add_m_ge [of 24 8 n] by simp
   done
 
-lemma [simp]: "and (((v::u64) >> 16) << 16) 16711680 = and v 16711680"
-  apply (simp add: bit_eq_iff)
-  apply (auto simp add: bit_simps)
+lemma u8_and_2_power_16_eq [bits_more_simp]: "and (((v::u64) >> 16) << 16) 16711680 = and v 16711680"
+  apply (auto simp add: bit_simps bit_eq_iff)
   subgoal for n using bit_power_k_add_m_ge [of 16 8 n] by simp
   subgoal for n using bit_power_k_add_m_ge [of 16 8 n] by simp
   done
 
-lemma [simp]: "and (((v::u64) >> 8) << 8) 65280 = and v 65280"
-  apply (simp add: bit_eq_iff)
-  apply (auto simp add: bit_simps)
+lemma u8_and_2_power_8_eq [bits_more_simp]: "and (((v::u64) >> 8) << 8) 65280 = and v 65280"
+  apply (auto simp add: bit_simps bit_eq_iff)
   subgoal for n using bit_power_k_add_m_ge [of 8 8 n] by simp
   subgoal for n using bit_power_k_add_m_ge [of 8 8 n] by simp
   done
 
-lemma bit_255_not_lt_64 : "n < 64 \<Longrightarrow>
+lemma bit_255_not_lt_64 [bits_more_simp]: "n < 64 \<Longrightarrow>
   \<not> bit (18374686479671623680::int) n \<Longrightarrow> \<not> bit (71776119061217280::int) n \<Longrightarrow>
   \<not> bit (280375465082880::int) n \<Longrightarrow> \<not> bit (1095216660480::int) n \<Longrightarrow>
   \<not> bit (4278190080::int) n \<Longrightarrow> \<not> bit (16711680::int) n \<Longrightarrow>
@@ -209,21 +178,18 @@ lemma bit_255_not_lt_64 : "n < 64 \<Longrightarrow>
   apply blast
   done
 
-lemma u64_of_u8_list_same: "(Some v = u64_of_u8_list l) = (l = u8_list_of_u64 v)"
+lemma u64_of_u8_list_same [bits_more_simp]: "(Some v = u64_of_u8_list l) = (l = u8_list_of_u64 v)"
   apply (unfold u64_of_u8_list_def u8_list_of_u64_def)
   apply (cases "length l \<noteq> 8", simp_all)
   subgoal by fastforce
   subgoal
     apply (rule iffI)
     subgoal
-      apply (simp add: u64_shl_shr_same u64_shl_shr_outside
-          u64_shl_shr_same_minus u64_and_or_255_same u64_ucast_and_ucast_255_same)
+      apply (simp add: bits_more_simp)
         using list_consists_8 by blast
 
     subgoal
-      apply (simp add: bit_eq_iff)
-      apply (simp add: bit_or_iff)
-      apply (auto simp add: bit_simps)
+      apply (auto simp add: bit_eq_iff bit_simps bits_more_simp)
       subgoal for n
         using bit_255_not_lt_64 by blast
       done
