theory/BitsOpMore4.thy
@@ -5,22 +5,11 @@ imports
 begin
 subsection \<open> u16_of_u8_list \<close>
 
-lemma ucast16_ucast8_and_255_eq [simp]: "ucast (((ucast (and v 255))::u8)) = and (v:: u16) 255"
-  apply (simp only: ucast_eq)
-(**r 
-word_of_int (uint (word_of_int (uint (and v 255)))) is
-
-(word_of_int (uint (and v 255)))::u8
-
-word_of_int (uint v_u8)  :: u64
-
-*)
-  apply (simp only: uint_word_of_int_eq word_and_def word_of_int_eq_iff)
-  apply (simp)
+lemma ucast16_ucast8_and_255_eq [bits_more_simp]: "ucast (((ucast (and v 255))::u8)) = and (v:: u16) 255"
+  apply (simp only: ucast_eq uint_word_of_int_eq word_and_def word_of_int_eq_iff)
   apply (simp add: bit_eq_iff)
   apply (auto simp add: bit_simps)
-  subgoal for n
-    apply (cases n, simp_all)
+  subgoal for n apply (cases n, simp_all)
     subgoal for n1 apply (cases n1, simp_all)
       subgoal for n2 apply (cases n2, simp_all)
         subgoal for n3 apply (cases n3, simp_all)
@@ -38,11 +27,9 @@ word_of_int (uint v_u8)  :: u64
     done
   done
 
-lemma u16_shl_shr_same: "n \<le> 8 \<Longrightarrow> ((ucast (v::u8) ::u16) << n) >> n = (ucast (v::u8) ::u16)"
-  apply (simp add: bit_eq_iff)
-  apply (auto simp add: bit_simps)
-  subgoal for k
-    apply (cases k, simp_all)
+lemma u16_shl_shr_same [bits_more_simp]: "n \<le> 8 \<Longrightarrow> ((ucast (v::u8) ::u16) << n) >> n = (ucast (v::u8) ::u16)"
+  apply (auto simp add: bit_simps bit_eq_iff)
+  subgoal for k apply (cases k, simp_all)
     subgoal for n1 apply (cases n1, simp_all)
       subgoal for n2 apply (cases n2, simp_all)
         subgoal for n3 apply (cases n3, simp_all)
@@ -60,27 +47,23 @@ lemma u16_shl_shr_same: "n \<le> 8 \<Longrightarrow> ((ucast (v::u8) ::u16) << n
     done
   done
 
-lemma u16_shl_shr_outside: "n+8 \<le> m \<Longrightarrow> ((ucast (v::u8) ::u16) << n) >> m = (0 ::u16)"
-  apply (simp add: bit_eq_iff)
-  apply (auto simp add: bit_simps u8_ge_8_bit_false)
-  done
+lemma u16_shl_shr_outside [bits_more_simp]: "n+8 \<le> m \<Longrightarrow> ((ucast (v::u8) ::u16) << n) >> m = (0 ::u16)"
+  by (auto simp add: bit_simps u8_ge_8_bit_false bit_eq_iff)
 
 lemma n_le_8_plus_lt_16: "(n::nat) \<le> 8 \<Longrightarrow> m \<le> n \<Longrightarrow> k < 16 \<Longrightarrow> n - m \<le> k \<Longrightarrow> k + m - n < 8 \<Longrightarrow> m + k < 16"
   by simp
 
-lemma u16_shl_shr_same_minus: "n \<le> 8 \<Longrightarrow> m \<le> n \<Longrightarrow>
+lemma u16_shl_shr_same_minus [bits_more_simp]: "n \<le> 8 \<Longrightarrow> m \<le> n \<Longrightarrow>
   ((ucast (v::u8) ::u16) << n) >> m = ((ucast (v::u8) ::u16) << (n-m))"
-  apply (simp add: bit_eq_iff)
-  apply (auto simp add: bit_simps u8_bit_true_ge_8 n_le_8_plus_lt_16)
+  apply (auto simp add: bit_simps u8_bit_true_ge_8 n_le_8_plus_lt_16 bit_eq_iff)
   subgoal for k
     by (simp add: add.commute)
   subgoal for k
     by (metis add.commute)
   done
 
-lemma u16_and_or_255_same: "8 \<le> n \<Longrightarrow> (and (or ((v::u16) << n) k) 255) = and k 255"
-  apply (simp add: bit_eq_iff)
-  apply (auto simp add: bit_simps)
+lemma u16_and_or_255_same [bits_more_simp]: "8 \<le> n \<Longrightarrow> (and (or ((v::u16) << n) k) 255) = and k 255"
+  apply (auto simp add: bit_simps bit_eq_iff)
   subgoal for t apply (cases t, simp_all)
     subgoal for n1 apply (cases n1, simp_all)
       subgoal for n2 apply (cases n2, simp_all)
@@ -99,12 +82,9 @@ lemma u16_and_or_255_same: "8 \<le> n \<Longrightarrow> (and (or ((v::u16) << n)
     done
   done
 
-lemma u16_ucast_and_ucast_255_same: "(ucast (and (ucast (v::u8)) (255::u16)) ::u8) = v"
-  apply (simp only: ucast_eq)
-  apply (simp only: uint_word_of_int_eq word_and_def word_of_int_eq_iff)
-  apply simp
-  apply (simp add: bit_eq_iff)
-  apply (auto simp add: bit_simps)
+lemma u16_ucast_and_ucast_255_same [bits_more_simp]: "(ucast (and (ucast (v::u8)) (255::u16)) ::u8) = v"
+  apply (simp only: ucast_eq uint_word_of_int_eq word_and_def word_of_int_eq_iff)
+  apply (auto simp add: bit_simps bit_eq_iff)
   subgoal for n apply (cases n, simp_all)
     subgoal for n1 apply (cases n1, simp_all)
       subgoal for n2 apply (cases n2, simp_all)
@@ -122,30 +102,27 @@ lemma u16_ucast_and_ucast_255_same: "(ucast (and (ucast (v::u8)) (255::u16)) ::u
   done
 
 
-lemma le_m_shr_0 : "8 \<le> m \<Longrightarrow> (ucast (v::u8) ::u16) >> m = (0 ::u16)"
-  apply (simp add: bit_eq_iff)
-  apply (auto simp add: bit_simps u8_ge_8_bit_false)
-  done
+lemma le_m_shr_0 [bits_more_simp]: "8 \<le> m \<Longrightarrow> (ucast (v::u8) ::u16) >> m = (0 ::u16)"
+  by (auto simp add: bit_simps u8_ge_8_bit_false bit_eq_iff)
 
 lemma list_consists_2 : "length l = 2 \<Longrightarrow> l = [l ! 0, l ! Suc 0]"
   by (metis Cons_nth_drop_Suc Suc_leI append.simps(1) drop_eq_Nil
       id_take_nth_drop lessI numeral_2_eq_2 take0 zero_less_Suc)
 
-lemma [simp]: "and (((v::u16) >> 8) << 8) 65280 = and v 65280"
-  apply (simp add: bit_eq_iff)
-  apply (auto simp add: bit_simps)
+lemma u16_and_2_power_8_eq [bits_more_simp]: "and (((v::u16) >> 8) << 8) 65280 = and v 65280"
+  apply (auto simp add: bit_simps bit_eq_iff)
   subgoal for n using bit_power_k_add_m_ge [of 8 8 n] by simp
   subgoal for n using bit_power_k_add_m_ge [of 8 8 n] by simp
   done
 
-lemma bit_255_not_lt_32 : "n < 16 \<Longrightarrow>
+lemma bit_255_not_lt_32 [bits_more_simp]: "n < 16 \<Longrightarrow>
   \<not> bit (65280::int) n \<Longrightarrow> bit (255::int) n"
   using bit_power_k_add_m_lt [of n 8  8] apply simp
   using bit_power_k_add_m_lt [of n 0  8] apply simp
   apply blast
   done
 
-lemma u16_of_u8_list_same: "(Some v = u16_of_u8_list l) = (l = u8_list_of_u16 v)"
+lemma u16_of_u8_list_same [bits_more_simp]: "(Some v = u16_of_u8_list l) = (l = u8_list_of_u16 v)"
   apply (unfold u16_of_u8_list_def u8_list_of_u16_def)
   apply (cases "length l \<noteq> 2", simp_all)
   subgoal by fastforce
@@ -154,8 +131,7 @@ lemma u16_of_u8_list_same: "(Some v = u16_of_u8_list l) = (l = u8_list_of_u16 v)
     subgoal
       apply simp
       apply (simp only: bit_eq_iff [of v])
-      apply (auto simp add: bit_simps u16_shl_shr_same u16_shl_shr_outside le_m_shr_0
-          u16_shl_shr_same_minus u16_and_or_255_same u16_ucast_and_ucast_255_same)
+      apply (auto simp add: bit_simps bits_more_simp)
 
       subgoal using list_consists_2
         by blast
@@ -164,7 +140,7 @@ lemma u16_of_u8_list_same: "(Some v = u16_of_u8_list l) = (l = u8_list_of_u16 v)
     subgoal
       apply (simp add: bit_eq_iff [of v])
       apply (simp add: bit_or_iff)
-      apply (auto simp add: bit_simps)
+      apply (auto simp add: bit_simps bits_more_simp)
       subgoal for n
         using bit_255_not_lt_32 by blast
       done
