theory/ListsMoreLemma.thy
@@ -1,0 +1,68 @@
+theory ListsMoreLemma
+imports
+  Main
+  rBPFCommType
+begin
+lemma l_0_and_1 [list_more_simp]: "l @ [a] = l_bin \<Longrightarrow> l_bin!(length l) = a" by fastforce
+lemma l_0_and_2 [list_more_simp]: "l @ [a, b] = l_bin \<Longrightarrow> l_bin!(length l) = a" by fastforce  
+lemma l_0_and_3 [list_more_simp]: "l @ [a, b, c] = l_bin \<Longrightarrow> l_bin!(length l) = a" by fastforce
+lemma l_0_and_4 [list_more_simp]: "l @ [a, b, c, d] = l_bin \<Longrightarrow> l_bin!(length l) = a" by fastforce
+lemma l_0_and_5 [list_more_simp]: "l @ [a, b, c, d, e] = l_bin \<Longrightarrow> l_bin!(length l) = a" by fastforce
+
+lemma l_1_and_2 [list_more_simp]: "l @ [a, b] = l_bin \<Longrightarrow> l_bin!(length l + 1) = b"
+  by (metis One_nat_def nth_Cons_0 nth_Cons_Suc nth_append_length_plus)
+lemma l_1_and_3 [list_more_simp]: "l @ [a, b, c] = l_bin \<Longrightarrow> l_bin!(length l + 1) = b"
+  by (metis One_nat_def nth_Cons_0 nth_Cons_Suc nth_append_length_plus)
+lemma l_1_and_4 [list_more_simp]: "l @ [a, b, c, d] = l_bin \<Longrightarrow> l_bin!(length l + 1) = b"
+  by (metis One_nat_def nth_Cons_0 nth_Cons_Suc nth_append_length_plus)
+lemma l_1_and_5 [list_more_simp]: "l @ [a, b, c, d, e] = l_bin \<Longrightarrow> l_bin!(length l + 1) = b"
+  by (metis One_nat_def nth_Cons_0 nth_Cons_Suc nth_append_length_plus)
+
+lemma l_1_and_2_S [list_more_simp]: "l @ [a, b] = l_bin \<Longrightarrow> l_bin!(Suc (length l)) = b"
+  by (metis One_nat_def add_diff_cancel_right' not_add_less2 nth_Cons_0 nth_Cons_Suc nth_append plus_1_eq_Suc)
+lemma l_1_and_3_S [list_more_simp]: "l @ [a, b, c] = l_bin \<Longrightarrow> l_bin!(Suc (length l)) = b"
+  by (metis One_nat_def add_diff_cancel_right' not_add_less2 nth_Cons_0 nth_Cons_Suc nth_append plus_1_eq_Suc)
+lemma l_1_and_4_S [list_more_simp]: "l @ [a, b, c, d] = l_bin \<Longrightarrow> l_bin!(Suc (length l)) = b"
+  by (metis One_nat_def add_diff_cancel_right' not_add_less2 nth_Cons_0 nth_Cons_Suc nth_append plus_1_eq_Suc)
+lemma l_1_and_5_S [list_more_simp]: "l @ [a, b, c, d, e] = l_bin \<Longrightarrow> l_bin!(Suc (length l)) = b"
+  by (metis One_nat_def add_diff_cancel_right' not_add_less2 nth_Cons_0 nth_Cons_Suc nth_append plus_1_eq_Suc)
+
+lemma l_2_and_3 [list_more_simp]: "l @ [a, b, c] = l_bin \<Longrightarrow> l_bin!(length l + 2) = c"
+  by (metis One_nat_def Suc_1 nth_Cons_0 nth_Cons_Suc nth_append_length_plus)
+lemma l_2_and_4 [list_more_simp]: "l @ [a, b, c, d] = l_bin \<Longrightarrow> l_bin!(length l + 2) = c"
+  by (metis One_nat_def Suc_1 nth_Cons_0 nth_Cons_Suc nth_append_length_plus)
+lemma l_2_and_5 [list_more_simp]: "l @ [a, b, c, d, e] = l_bin \<Longrightarrow> l_bin!(length l + 2) = c"
+  by (metis One_nat_def Suc_1 nth_Cons_0 nth_Cons_Suc nth_append_length_plus)
+
+
+lemma l_2_and_3_S [list_more_simp]: "l @ [a, b, c] = l_bin \<Longrightarrow> l_bin!(Suc (Suc (length l))) = c"
+  by (metis Cons_eq_appendI One_nat_def add_Suc_right append_Nil length_append list.size(3) list.size(4) nth_append_length nth_append_length_plus plus_1_eq_Suc)
+lemma l_2_and_4_S [list_more_simp]: "l @ [a, b, c, d] = l_bin \<Longrightarrow> l_bin!(Suc (Suc (length l))) = c"
+  by (metis Cons_eq_appendI One_nat_def add_Suc_right append_Nil length_append list.size(3) list.size(4) nth_append_length nth_append_length_plus plus_1_eq_Suc)
+lemma l_2_and_5_S [list_more_simp]: "l @ [a, b, c, d, e] = l_bin \<Longrightarrow> l_bin!(Suc (Suc (length l))) = c"
+  by (metis Cons_eq_appendI One_nat_def add_Suc_right append_Nil length_append list.size(3) list.size(4) nth_append_length nth_append_length_plus plus_1_eq_Suc)
+
+lemma l_3_and_4 [list_more_simp]: "l @ [a, b, c, d] = l_bin \<Longrightarrow> l_bin!(length l + 3) = d"
+  by force
+lemma l_3_and_5 [list_more_simp]: "l @ [a, b, c, d, e] = l_bin \<Longrightarrow> l_bin!(length l + 3) = d"
+  by force
+
+
+lemma l_3_and_4_S [list_more_simp]: "l @ [a, b, c, d] = l_bin \<Longrightarrow> l_bin!(Suc (Suc (Suc (length l)))) = d"
+  by (metis One_nat_def Suc3_eq_add_3 add_diff_cancel_right' last.simps last_conv_nth length_Cons list.discI list.size(3) not_add_less2 nth_append)
+lemma l_3_and_5_S [list_more_simp]: "l @ [a, b, c, d, e] = l_bin \<Longrightarrow> l_bin!(Suc (Suc (Suc (length l)))) = d"
+  by (metis Suc3_eq_add_3 add.commute nth_Cons_0 nth_Cons_Suc nth_append_length_plus numeral_3_eq_3)
+
+lemma l_4_and_5 [list_more_simp]: "l @ [a, b, c, d, e] = l_bin \<Longrightarrow> l_bin!(length l + 4) = e"
+  by force
+
+lemma l_4_and_5_S [list_more_simp]: "l @ [a, b, c, d, e] = l_bin \<Longrightarrow> l_bin!(Suc (Suc (Suc (Suc (length l))))) = e"
+  by (metis Nil_is_append_conv One_nat_def Suc_1 add_2_eq_Suc' add_Suc_right diff_Suc_1' last.simps last_appendR last_conv_nth length_Cons length_append list.discI list.size(3))
+
+lemma l_1_len_1 [list_more_simp]: "l @ [a] = l_bin \<Longrightarrow> length l_bin - length l = 1" by fastforce
+lemma l_1_len_2 [list_more_simp]: "l @ [a, b] = l_bin \<Longrightarrow> length l_bin - length l = 2" by fastforce  
+lemma l_1_len_3 [list_more_simp]: "l @ [a, b, c] = l_bin \<Longrightarrow> length l_bin - length l = 3" by fastforce
+lemma l_1_len_4 [list_more_simp]: "l @ [a, b, c, d] = l_bin \<Longrightarrow> length l_bin - length l = 4" by fastforce
+lemma l_1_len_5 [list_more_simp]: "l @ [a, b, c, d, e] = l_bin \<Longrightarrow> length l_bin - length l = 5" by fastforce
+
+end
