theory/x64DecodeProof1.thy
@@ -1,0 +1,37 @@
+theory x64DecodeProof1
+imports
+  Main
+  rBPFCommType x86CommType
+  x64Assembler x64Disassembler
+begin
+
+lemma list_nth_right: "v = l!n \<Longrightarrow> l!n = v" using HOL.sym by simp
+
+lemma if_false_eq: "a \<noteq> b \<Longrightarrow> (if a = b then c else d) = d" using HOL.if_not_P
+  by argo 
+
+lemma construct_rex_to_u8_neq_144: "construct_rex_to_u8 b0 b1 b2 b3 \<noteq> 144"
+  apply (unfold construct_rex_to_u8_def bitfield_insert_u8_def Let_def u8_of_bool_def)
+  apply (cases b0; cases b1; cases b2; cases b3; simp)
+  done
+
+lemma x64_encode_decode_consistency:
+  "list_in_list l_bin pc l \<Longrightarrow> Some l_bin = x64_encode ins \<Longrightarrow>
+    x64_decode pc l = Some (length l_bin, ins)"
+  apply (cases ins; simp add: Let_def)
+
+  subgoal for rd rs
+    apply (simp add: split: if_split_asm; erule conjE)
+    subgoal
+      apply (drule HOL.sym [of _ "l ! Suc pc"])
+      apply (simp add: x64_decode_def
+          bitfield_extract_u8_def bitfield_insert_u8_def ireg_of_u8_def)
+      apply (simp add: Let_def)
+(*
+    apply (cases ins; simp add: Let_def construct_rex_to_u8_neq_144) *)
+(*
+  apply (subst if_false_eq, simp) *)
+
+
+
+end
