ROOT
@@ -1,4 +1,4 @@
 session Solana_rBPF = Main +
-  options [timeout = 600]
+  options [timeout = 600, threads=16]
   theories
     rBPFSyntax
